add equivalence tag function and kvstore delete/insert

src/coupon_collector/EvolvedCouponCollector.lean
@@ -21,6 +21,62 @@ structure KVStore where
  | Request.Symmetry t       => some ({lhs := t.rhs, rhs := t.lhs})
  | Request.Transitivity t₁ t₂ => if t₁.rhs == t₂.lhs then some {lhs := t₁.lhs, rhs := t₂.rhs} else none
  
+/-
+Two ways to get an equivalence tag: from Tag struct or from KVStore
+Enforcing how KVStore should be updated: only when it doesn't break equivalence tag
+-/
+-- equivalenceTag function to issue a tag: assuming the keys already exist in the store
+
+-- bypassing coupon collector to get a tag
+def issue_equivalence_tag (store : KVStore) (lhs rhs : String) : Option Tag :=
+  if store.mapping lhs == store.mapping rhs then
+    some { lhs := lhs, rhs := rhs }
+  else
+    none
+
+-- via coupon collector to get equivalence tag
+def Tag.EquivalenceInvariant (store : KVStore)(t : Tag) : Bool := 
+  store.mapping t.lhs == store.mapping t.rhs
+
+def request_equivalence_tag (store : KVStore) (r : Request) : Option Tag :=
+  match apply_coupon_collector r with
+  | some t => if Tag.EquivalenceInvariant store t then some t else none
+  | none => none
+
+-- we don't want KVStore to delete a key if the key is still pointing to the value 
+-- or inserting a new key with same name as existing key but points to a diff value
+def KVStore.insert (store : KVStore) (key : String) (val : Nat) : Bool := 
+  match store.mapping key with 
+  | none => true
+  | some existing_val => existing_val == val 
+
+-- return an updated store after deletion 
+def KVStore.delete (store : KVStore) (key : String) : Option KVStore := 
+  match store.mapping key with 
+  | none => none 
+  | some _ => 
+      some {
+        mapping := λ k => 
+          if k == key then none else store.mapping k 
+      }
+
+-- some test cases of the functions above:  
+def test_store : KVStore := 
+  {mapping := λ key => 
+  if key = "a" then some 42
+  else if key = "b" then some 42 
+  else if key = "c" then some 5
+  else none}
+#eval issue_equivalence_tag test_store "a" "b"
+#eval request_equivalence_tag test_store (Request.Identity "a")
+#eval request_equivalence_tag test_store (Request.Symmetry {lhs := "a", rhs :="b"})
+#eval KVStore.insert test_store "d" 1
+#eval match KVStore.delete test_store "b" with
+  | some newStore => newStore.mapping "a"  -- should be none
+  | none => none
+-- coupon collector trusts the authorship 
+-- store should be trusted: what is store responsible for? 
+-- keys cann be inseted/deleted 
 
 def Request.toList : Request -> List Tag
   | Request.Identity _ => []
@@ -28,13 +84,13 @@ def Request.toList : Request -> List Tag
   | Request.Transitivity t₁ t₂ => [t₁, t₂]
 
 def all_tag_true (store : KVStore) (ts: List Tag) : Bool :=
-  ts.all λ t => store.mapping t.lhs == store.mapping t.rhs
+  ts.all λ t => store.mapping t.lhs == store.mapping t.rhs -- runtime check 
 
 
 theorem soundness_proof : 
   ∀ (r : Request), ∀ (store : KVStore),
     all_tag_true store r.toList  →
-    all_tag_true store (Option.toList (apply_coupon_collector r)) := by
+    all_tag_true store (Option.toList (apply_coupon_collector r)) := by -- apply_coupon_collector r.toList
   intros r store h 
   cases r with 
     | Identity x => 
@@ -52,7 +108,6 @@ theorem soundness_proof :
           simp [h₁, h₂]
         | some v₁ =>
           simp [h₁, h₂] at h
-
       | some v₂ =>
         cases h₂ : store.mapping t.rhs with
         | none =>
